lib_avl_mono/Impl.Trees.Rotate2.M.fst
@@ -14,15 +14,14 @@ module U32 = FStar.UInt32
 open Spec.Trees
 open Impl.Core
 open Impl.Common
+open Impl.Trees.Types
 open Impl.Trees.M
 
 #set-options "--fuel 0 --ifuel 0 --ide_id_info_off"
 
-let a = Impl.Trees.M.a
-
 #push-options "--fuel 1 --ifuel 1 --z3rlimit 50"
-let rotate_right_left (ptr: t a)
-  : Steel (t a)
+let rotate_right_left (ptr: t)
+  : Steel t
   (linked_tree ptr)
   (fun ptr' -> linked_tree ptr')
   (requires (fun h0 ->
